Simplified decode; seeing something that looks like magic or inconsistency

examples/algorithms/Huffman.fst
@@ -5,6 +5,9 @@ open FStar.List.Tot
 
 type symbol = char
 
+// TODO: could move weights away from the nodes,
+// only need one weight per each trie in the forest
+
 type trie =
   | Leaf : w:pos -> s:symbol -> trie
   | Node : w:pos -> l:trie -> r:trie -> trie
@@ -20,7 +23,7 @@ let leq_trie (t1:trie) (t2:trie) : Tot bool =
 let rec sorted (ts:list trie) : Tot bool=
   match ts with
   | [] | [_] -> true
-  | t1::t2::ts' -> (leq_trie t1 t1) && (sorted (t2::ts'))
+  | t1::t2::ts' -> leq_trie t1 t1 && sorted (t2::ts')
 
 let rec insert_in_sorted (x:trie) (xs:list trie) : Pure (list trie)
     (requires (b2t (sorted xs)))
@@ -28,8 +31,8 @@ let rec insert_in_sorted (x:trie) (xs:list trie) : Pure (list trie)
            /\ List.Tot.length ys == List.Tot.length xs + 1)) =
   match xs with
   | [] -> [x]
-  | x'::xs' -> if weight x < weight x' then (admit(); x :: xs)
-               else (admit(); x' :: (insert_in_sorted x xs'))
+  | x'::xs' -> if leq_trie x x' then x :: xs
+               else x' :: (insert_in_sorted x xs')
 
 let rec insertion_sort (ts : list trie) : Pure (list trie)
     (requires (True)) (ensures (fun ts -> sorted ts)) =
@@ -37,18 +40,43 @@ let rec insertion_sort (ts : list trie) : Pure (list trie)
   | [] -> []
   | t::ts' -> insert_in_sorted t (insertion_sort ts')
 
+let rec lemma_that_needs_induction (w:pos) (t1:trie) (t2:trie) (ts:list trie) :
+  Lemma
+    (requires (b2t (sorted ts)))
+    (ensures (sorted ts ==> (* without sorted the error message is amazing! *)
+              existsb #trie is_Node ((Node w t1 t2) `insert_in_sorted` ts)))
+    (decreases ts) =
+  match ts with
+    | [] -> ()
+    | t::ts' -> if leq_trie (Node w t1 t2) t then ()
+                else lemma_that_needs_induction w t1 t2 ts'
+
+(* TODO: This magically derives lemma_that_needs_induction? WTF? *)
 let rec huffman_trie (ts:list trie) : Pure trie
     (requires (sorted ts /\ List.Tot.length ts > 0))
-    (ensures (fun cs -> True)) (decreases (List.Tot.length ts)) =
+    (ensures (fun t ->
+      (List.Tot.length ts > 1 \/ existsb is_Node ts ==> is_Node t)))
+    (decreases (List.Tot.length ts)) =
   match ts with
   | t1::t2::ts' ->
+      assert(List.Tot.length ts > 1); (* so it needs to prove is_Node for t *)
       let w = weight t1 + weight t2 in
-      huffman_trie (Node w t1 t2 `insert_in_sorted` ts')
+      let t = huffman_trie (Node w t1 t2 `insert_in_sorted` ts') in
+      (* by the recursive call we know:
+         (List.Tot.length (Node w t1 t2 `insert_in_sorted` ts') > 1
+          \/ existsb is_Node (Node w t1 t2 `insert_in_sorted` ts') ==> is_Node t) *)
+      (* I think tht the only way we can use this is by proving:
+          existsb is_Node (Node w t1 t2 `insert_in_sorted` ts') *)
+      (* but somehow F* manages to prove this without! the following assert fails
+         without lemma_that_needs_induction (but works with it)
+         lemma_that_needs_induction w t1 t2 ts';
+         assert(existsb is_Node (Node w t1 t2 `insert_in_sorted` ts')); *)
+      t
   | [t1] -> t1
 
 let huffman (sws:list (symbol*pos)) : Pure trie
     (requires (b2t (List.Tot.length sws > 0)))
-    (ensures (fun _ -> True)) =
+    (ensures (fun t -> List.Tot.length sws > 1 ==> is_Node t)) =
   huffman_trie (insertion_sort (List.Tot.map (fun (s,w) -> Leaf w s) sws))
 
 let rec encode_one (t:trie) (s:symbol) : Tot (option (list bool)) =
@@ -68,6 +96,8 @@ let rec encode (t:trie) (ss:list symbol) : Tot (option (list bool)) =
   | s::ss' -> match encode_one t s, encode t ss' with
               | Some bs, Some bs' -> Some (bs @ bs')
               | _, _ -> None
+
+// A more complex decode I originally wrote
 
 let rec decode_one (t:trie) (bs:list bool) : Pure (option (symbol * list bool))
     (requires (True))
@@ -91,13 +121,31 @@ let rec decode (t:trie) (bs:list bool) : Tot (option (list symbol))
                                             | None    -> None)
                         | _ -> None
 
+// Simplified decode using idea from Bird and Wadler's book
+
+let rec decode_aux (t':trie) (t:trie) (bs:list bool) : Pure (option (list symbol))
+    (requires (b2t (is_Node t'))) (ensures (fun _ -> True))
+    (decreases (%[bs; if is_Leaf t && is_Cons bs then 1 else 0]))
+  =
+  match t, bs with
+  | Leaf _ s, [] -> Some [s]
+  | Leaf _ s, _::_ -> (match decode_aux t' t' bs with
+                      | Some ss -> Some (s :: ss)
+                      | None -> None)
+  | Node _ t1 t2, b :: bs' -> decode_aux t' (if b then t2 else t1) bs'
+  | Node _ _ _, [] -> None
+
+let decode' (t:trie) (bs:list bool) : Pure (option (list symbol))
+    (requires (b2t (is_Node t))) (ensures (fun _ -> True)) =
+  decode_aux t t bs
+
 // proving this should require prefix freedom
 let cancelation (sws:list (symbol*pos)) (ss:list symbol) : Lemma
   (requires (b2t (List.Tot.length sws > 0)))
-  (ensures (List.Tot.length sws > 0 ==>
+  (ensures (List.Tot.length sws > 1 ==>
             (let t = huffman sws in
             (match encode t ss with
-            | Some e -> (match decode t e with
+            | Some e -> (match decode' t e with
                         | Some d -> d = ss
                         | None -> True)
             | None -> True)))) = admit()
